work

LTS.thy
@@ -2,10 +2,12 @@ theory LTS imports Transition_Systems_and_Automata.Transition_System_Constructio
 
 type_synonym ('state, 'label) transition = "'state * 'label * 'state"
 
+
 locale LTS =
   fixes transition_relation :: "('state, 'label) transition set"
-    and r :: 'state
 begin
+
+text \<open>We define execution and what it means to be enabled.\<close>
 
 fun execute :: "('state, 'label) transition \<Rightarrow> 'state \<Rightarrow> 'state" where 
   "execute (s, l, s') s'' = s'"
@@ -13,10 +15,248 @@ fun execute :: "('state, 'label) transition \<Rightarrow> 'state \<Rightarrow> '
 fun enabled :: "('state, 'label) transition \<Rightarrow> 'state \<Rightarrow> bool" where
   "enabled (s, l, s') s'' \<longleftrightarrow> (s, l, s') \<in> transition_relation \<and> s = s''"
 
-interpretation transition_system execute enabled .
+text \<open>We interpret transition_system_initial.\<close>
+
+interpretation ts: transition_system execute enabled .
 
 
+find_theorems execute
+
+text \<open>We "open" the interpretation.\<close>
+
+abbreviation successors :: "'state \<Rightarrow> 'state set" where
+   "successors == ts.successors"
+
+abbreviation path :: "('state, 'label) transition list \<Rightarrow> 'state \<Rightarrow> bool" where 
+  "path s p == ts.path s p" (* s is a path from p. *)
+
+abbreviation run :: "('state, 'label) transition stream \<Rightarrow> 'state \<Rightarrow> bool" where 
+  "run == ts.run"
+
+abbreviation reachable :: "'state \<Rightarrow> 'state set" where
+  "reachable == ts.reachable"
+
+abbreviation reachablep :: "'state \<Rightarrow> 'state \<Rightarrow> bool" where
+  "reachablep == ts.reachablep"
+
+text \<open>More definitions.\<close>
+
+(* Paths as defined in the thesis: *)
+inductive_set spath :: "'state list set" where
+  "[] \<in> spath"
+| "[s] \<in> spath"
+| "(s'#ss) \<in> spath \<Longrightarrow> (s,l,s') \<in> transition_relation \<Longrightarrow> (s#s'#ss) \<in> spath"
+
+(* Labeled paths as defined in the thesis *)
+inductive_set lspath :: "('state * 'label list * 'state) set" where
+  transition_star_refl[iff]: "(p, [], p) \<in> lspath"
+| transition_star_step: "\<lbrakk>(p,\<gamma>,q') \<in> t; (q',w,q) \<in> lspath\<rbrakk>
+                           \<Longrightarrow> (p, \<gamma>#w, q) \<in> lspath"
+
+(* TODO: Prove correspondences between spath, path and lspath.
+   "Lift" path's theorem to spath and lspath
+ *)
+
+abbreviation transition_star :: "('state \<times> 'label list \<times> 'state) set" where (* Morten terminology -- but I dropped the transition set *)
+  "transition_star \<equiv> lspath"
+
+(* lemma transition_star_mono[mono]: "mono transition_star" *) (* Not possible with my definition of transition_star *)
 
 end
+
+locale LTS_init = LTS transition_relation for transition_relation :: "('state, 'label) transition set" +
+  fixes r :: 'state
+begin
+
+text \<open>We interpret transition_system_initial.\<close>
+
+interpretation ts: transition_system_initial execute enabled "\<lambda>r'. r' = r" .
+
+text \<open>We "open" the interpretation.\<close>
+
+abbreviation nodes :: "'state set" where
+  "nodes == ts.nodes"
+
+end
+
+datatype 'label operation = pop | swap 'label | push 'label 'label
+type_synonym ('ctr_loc, 'label) rule = "('ctr_loc \<times> 'label) \<times> ('ctr_loc \<times> 'label operation)"
+type_synonym ('ctr_loc, 'label) conf = "'ctr_loc \<times> 'label list"
+
+text \<open>We define push down systems.\<close>
+
+locale PDS =
+  (* 'ctr_loc is the type of control locations *)
+  fixes P_locs :: "'ctr_loc set" 
+    and \<Gamma> :: "'label set"
+    and \<Delta> :: "('ctr_loc, 'label) rule set"
+    and c0 :: "('ctr_loc, 'label) conf"
+  assumes "\<Delta> \<subseteq> (P_locs \<times> UNIV) \<times> (P_locs \<times> UNIV)"
+begin
+
+fun config_wf :: "('ctr_loc, 'label) conf \<Rightarrow> bool" where
+  "config_wf (c, l) \<longleftrightarrow> c \<in> P_locs"
+
+primrec op_labels :: "'label operation \<Rightarrow> 'label list" where
+  "op_labels pop = []"
+| "op_labels (swap \<gamma>) = [\<gamma>]" 
+| "op_labels (push \<gamma>  \<gamma>') = [\<gamma>, \<gamma>']"
+
+definition is_rule :: "'ctr_loc \<times> 'label \<Rightarrow> 'ctr_loc \<times> 'label operation \<Rightarrow> bool" (infix "\<hookrightarrow>" 80) where
+  "x \<hookrightarrow> y \<equiv> (x,y) \<in> \<Delta>"
+
+inductive_set transition_rel :: "(('ctr_loc, 'label) conf \<times> 'label \<times> ('ctr_loc, 'label) conf) set" where
+  "(p, \<gamma>) \<hookrightarrow> (p', w) \<Longrightarrow> ((p, \<gamma>#w'), \<gamma>, (p', (op_labels w)@w')) \<in> transition_rel"
+
+text \<open>We interpret LTS.\<close>
+
+interpretation pds: LTS_init transition_rel c0 .
+(* Det er måske lidt problematisk at P_locs ikke bliver sendt der ind. *)
+
+text \<open>We "open" the interpretation.\<close>
+
+abbreviation pds_execute :: "(('ctr_loc, 'label) conf, 'label) transition \<Rightarrow> ('ctr_loc, 'label) conf \<Rightarrow> ('ctr_loc, 'label) conf" where
+  "pds_execute == pds.execute"
+
+abbreviation pds_enabled :: "(('ctr_loc, 'label) conf, 'label) transition \<Rightarrow> ('ctr_loc, 'label) conf \<Rightarrow> bool" where
+  "pds_enabled == pds.enabled"
+
+abbreviation pds_successors :: "('ctr_loc, 'label) conf \<Rightarrow> ('ctr_loc, 'label) conf set" where
+  "pds_successors == pds.successors"
+
+abbreviation "pds_step == pds_successors" (* Morten/Stefan terminology *)
+
+abbreviation pds_path :: "(('ctr_loc, 'label) conf, 'label) transition list \<Rightarrow> ('ctr_loc, 'label) conf \<Rightarrow> bool" where
+  "pds_path == pds.path"
+
+abbreviation pds_run :: "(('ctr_loc, 'label) conf, 'label) transition stream \<Rightarrow> ('ctr_loc, 'label) conf \<Rightarrow> bool" where
+  "pds_run == pds.run"
+
+abbreviation pds_reachable :: "('ctr_loc, 'label) conf \<Rightarrow> ('ctr_loc, 'label) conf set" where
+  "pds_reachable == pds.reachable"
+
+abbreviation pds_reachablep :: "('ctr_loc, 'label) conf \<Rightarrow> ('ctr_loc, 'label) conf \<Rightarrow> bool" (infix "\<Rightarrow>\<^sup>*" 80) where
+  "c \<Rightarrow>\<^sup>* c' == pds.reachablep c c'"
+
+
+abbreviation pds_nodes :: "('ctr_loc, 'label) conf set" where
+  "pds_nodes == pds.nodes"
+
+definition pds_step_relp  :: "('ctr_loc, 'label) conf \<Rightarrow> ('ctr_loc, 'label) conf \<Rightarrow> bool" (infix "\<Rightarrow>" 80) where
+  "c \<Rightarrow> c' \<equiv> c' \<in> pds_successors c"
+
+definition psd_spath :: " ('ctr_loc, 'label) conf list set" where
+  "psd_spath \<equiv> pds.spath"
+
+definition psd_lspath :: "(('ctr_loc, 'label) conf \<times> 'label list \<times> ('ctr_loc, 'label) conf) set" where
+  "psd_lspath \<equiv> pds.lspath"
+
+
+text \<open>More definitions\<close>
+
+abbreviation "pds_step_starp == pds_reachablep" (* Morten/Stefan terminology *) (* TODO: copy into LTS *)
+
+definition pds_step_rel :: "('ctr_loc, 'label) conf rel" where (* TODO: copy into LTS *)
+  "pds_step_rel \<equiv> {(c, c'). pds_step_relp c c'}"
+
+definition pds_step_star :: "('ctr_loc, 'label) conf rel" where (* TODO: copy into LTS *)
+  "pds_step_star \<equiv> {(c, c'). pds_step_starp c c'}"
+
+abbreviation
+  pds_step_star_trans ("(_\<Rightarrow>\<^sup>*_\<Rightarrow>\<^sup>*_)" 80) where (* TODO: copy into LTS *)
+  "c \<Rightarrow>\<^sup>* c' \<Rightarrow>\<^sup>* c'' \<equiv> (c \<Rightarrow>\<^sup>* c') \<and> (c' \<Rightarrow>\<^sup>* c'')"
+
+(* For a set of configurations C, post*(C) is the set of all configurations reachable from C. *) (* TODO: copy into LTS *)
+definition pds_post_star :: "('ctr_loc, 'label) conf set \<Rightarrow> ('ctr_loc, 'label) conf set" where
+  "pds_post_star C \<equiv> {c'. \<exists>c \<in> C. c \<Rightarrow>\<^sup>* c'}"
+
+(* And pre*(C) is the set of all configurations that can reach a configuration in C. *)  (* TODO: copy into LTS *)
+definition pds_pre_star :: "('ctr_loc, 'label) conf set \<Rightarrow> ('ctr_loc, 'label) conf set" where
+  "pds_pre_star C \<equiv> {c'. \<exists>c \<in> C. c' \<Rightarrow>\<^sup>* c}"
+
+end
+
+locale PDS_with_P_automaton = PDS P_locs \<Gamma>
+  for P_locs :: "'ctr_loc set" 
+    and \<Gamma> :: "'label set"
+    +
+  fixes Q_locs :: "'ctr_loc set" 
+    and trans :: "('ctr_loc, 'label) transition set" 
+    and F_locs :: "'ctr_loc set"
+  assumes "P_locs \<subseteq> Q_locs"
+    and "trans \<subseteq> Q_locs \<times> UNIV \<times> Q_locs"
+    and "F_locs \<subseteq> Q_locs"
+begin
+
+interpretation autom: LTS trans .
+
+
+text \<open>We "open" the interpretation.\<close>
+abbreviation autom_execute :: "('ctr_loc, 'label) transition \<Rightarrow> 'ctr_loc \<Rightarrow> 'ctr_loc" where 
+  "autom_execute \<equiv> autom.execute"
+
+abbreviation autom_enabled :: "('ctr_loc, 'label) transition \<Rightarrow> 'ctr_loc \<Rightarrow> bool" where 
+  "autom_enabled  \<equiv> autom.enabled"
+
+abbreviation autom_successors :: "'ctr_loc \<Rightarrow> 'ctr_loc set" where 
+   "autom_successors \<equiv> autom.successors"
+
+abbreviation autom_path :: "('ctr_loc, 'label) transition list \<Rightarrow> 'ctr_loc \<Rightarrow> bool" where
+  "autom_path \<equiv> autom.path"
+
+abbreviation autom_run  :: "('ctr_loc, 'label) transition stream \<Rightarrow> 'ctr_loc \<Rightarrow> bool" where
+  "autom_run \<equiv> autom.run"
+
+abbreviation autom_reachable :: "'ctr_loc \<Rightarrow> 'ctr_loc set" where
+  "autom_reachable \<equiv> autom.reachable"
+
+abbreviation autom_reachablep :: "'ctr_loc \<Rightarrow> 'ctr_loc \<Rightarrow> bool" where 
+  "autom_reachablep \<equiv> autom.reachablep"
+
+abbreviation autom_spath :: "'ctr_loc list set" where
+  "autom_spath \<equiv> autom.spath"
+
+abbreviation autom_lspath :: "('ctr_loc * 'label list * 'ctr_loc) set" where
+  "autom_lspath \<equiv> autom.lspath"
+
+abbreviation autom_transition_star :: "('ctr_loc \<times> 'label list \<times> 'ctr_loc) set" where 
+  "autom_transition_star \<equiv> autom.transition_star"
+
+text \<open>More definitions\<close>
+
+fun accepts :: "('ctr_loc, 'label) conf \<Rightarrow> bool" where
+  "accepts (p,l) \<longleftrightarrow> (\<exists>q \<in> F_locs. (p,l,q) \<in> autom_lspath)" 
+(* Here acceptance is defined for any p, but in the paper p has to be in P_locs *)
+
+(* Potentially useful lemmas. *)
+
+(* lemma accepts_mono[mono]: "mono accepts" *) (* Not possible with my definition of transition_star *)
+
+lemma accepts_cons: "(p, \<gamma>, q) \<in> trans \<Longrightarrow> accepts (q, w) \<Longrightarrow> accepts (p, \<gamma> # w)"
+  by (meson accepts.simps autom.lspath.intros(2))
+
+lemma accepts_unfold: "accepts (p, \<gamma> # w) \<Longrightarrow> \<exists>q. (p, \<gamma>, q) \<in> trans \<and> accepts (q, w)"
+proof -
+  assume "accepts (p, \<gamma> # w)"
+  then obtain q where "q \<in> F_locs \<and> (p,\<gamma> # w,q) \<in> autom_lspath"
+    by auto
+  find_theorems autom_lspath
+
+  have "(p, \<gamma>, q') \<in> trans \<and> accepts (q', w)"
+  
+  show "\<exists>q. (p, \<gamma>, q) \<in> trans \<and> accepts (q, w)"
+    sorry
+qed
+
+
+
+
+
+
+
+
+
+
+
 
 end
